Renest.v
@@ -1,0 +1,431 @@
+Require Import AllInRel Util Map Env EnvTy Exp IL Bisim DecSolve MoreList InRel Sublist.
+
+Set Implicit Arguments.
+Unset Printing Records.
+
+(** Pull all definitions to the top.
+    [D] at index f holds the new index of function f
+    n is the number of pulled-up defintions so far (n >= length D),
+    not neccessarily equal
+    yields the transformed statement and the global definitions
+*)
+
+Definition egalize_funs (egalize:list nat -> nat -> stmt -> stmt * list (params * stmt))
+           (D':list nat) (n:nat) (F:list (params * stmt)) :=
+  fold_right (fun f nF' =>
+                       let '(n, F1, F2) := nF' in
+                       let (s, F'') := egalize D' n (snd f) in
+                       let n' := n + length F'' in
+                       (n', (fst f, s)::F1, F2 ++ F'')) (n, nil, nil) F.
+
+Definition extend n (F:list (params * stmt)) D := mapi (fun i _ => i+n) F ++ D.
+
+Fixpoint egalize (D:list nat) (n:nat) (s:stmt) : stmt * list (params * stmt) :=
+  match s with
+    | stmtLet x e s =>
+      let (s', F) := egalize D n s in
+      (stmtLet x e s', F)
+    | stmtExtern x f Y s =>
+      let (s', F) := egalize D n s in
+      (stmtExtern x f Y s', F)
+    | stmtIf x s1 s2 =>
+      let (s1', F1) := egalize D n s1 in
+      let (s2', F2) := egalize D (n + length F1) s2 in
+      (stmtIf x s1' s2', F1 ++ F2)
+    | stmtApp l Y => (stmtApp (LabI (nth (counted l) D 0)) Y, nil)
+    | stmtReturn x => (stmtReturn x, nil)
+    | stmtFun F s =>
+      (* entries for definitions in F: they are put to the bottom of the stack *)
+      let D' := extend n F D in
+      let '(n', F1, F2) := egalize_funs egalize D' (length F + n) F in
+      let (s', F'') := egalize D' n' s in
+      (s', F1 ++ F2 ++ F'')
+  end.
+
+(*
+Lemma foo L
+ :
+  (forall f b, get L f b -> f > block_n b)
+-> (forall f n b b', get L f b -> get L (f - block_n b + n) b' -> n > block_n b').
+Proof.
+  intros.
+  eapply H in H0. eapply H in H1. simpl in *.
+Qed.
+*)
+(*
+Lemma inRel_resetting {A} {B} `{BlockType B} {C} `{BlockType C} R
+      (AL:list A) (L:list B) (L':list C)
+: inRel R AL L L' -> n_resetting L.
+Proof.
+  intros. unfold n_resetting.
+  general induction H1. inv H2; eauto.
+  eapply get_app_cases in H3; destruct H3; dcr;
+  eapply get_app_cases in H4; destruct H4; dcr.
+  - erewrite mutual_block_zero; eauto.
+    erewrite mutual_block_zero; eauto. omega.
+  - exploit (eapply (mutual_block_zero H2); eauto).
+    exploit (eapply (inRel_less H1 H5)). omega.
+  - exploit (eapply (inRel_less H1 H5)).
+    exploit (eapply (get_length H3)). omega.
+  - eapply IHinRel.  eapply H5.
+    exploit (eapply (inRel_less H1 H5)).
+    orewrite (f - length L1' - block_n b + n = f - block_n b + n - length L1'); eauto.
+Qed.
+*)
+(*
+Definition n_smaller' n L :=
+        forall f b, get L f b -> (f+n) >= I.block_n b.
+
+Definition n_resetting' m {B} `{BlockType B} (L:list B) :=
+  (forall f n b b', get L f b -> get L (f - block_n b + n) b' -> (n+m) >= block_n b').
+
+
+
+Lemma sawtooth_invariant L F n
+  : n_smaller' n L -> n_resetting' n L
+    -> n_smaller' n (mapi_impl I.mkBlock n F ++ L).
+Proof.
+  general induction F; simpl; eauto.
+  exploit (eapply (IHF L (S n))); eauto.
+  - hnf; intros. specialize (H _ _ H1). omega.
+  - hnf; intros. specialize (H0 _ _ _ _ H1 H2). omega.
+  - hnf; intros. inv H1. simpl; omega.
+    specialize (X _ _ H6). omega.
+Qed.
+*)
+(*
+Definition sawtooth B `{BlockType B} (L:list B) :=
+  forall f b b', get L f b -> get L (S f) b' -> S (block_n b) = block_n b' \/ block_n b' = 0.
+
+Definition sawtooth_n B `{BlockType B} n (L:list B)
+ := sawtooth L /\ forall b, get L 0 b -> block_n b = n.
+
+
+Lemma sawtooth_I_mkBlock' L F n
+  : sawtooth_n 0 L
+    -> sawtooth (mapi_impl I.mkBlock n F ++ L).
+Proof.
+  unfold sawtooth_n.
+  general induction F; simpl in * |- *; eauto. eapply H; eauto.
+  hnf; intros. inv H0; inv H1. simpl.
+  destruct F; simpl in *. right. eapply H; eauto.
+  left. inv H6. simpl. reflexivity.
+  eapply IHF; eauto.
+Qed.
+
+
+Lemma sawtooth_I_mkBlock L F
+  : sawtooth_n 0 L
+    -> sawtooth_n 0 (mapi_impl I.mkBlock 0 F ++ L).
+Proof.
+  split; eauto using sawtooth_I_mkBlock'.
+  intros. destruct F; simpl in *.
+  - eapply H; eauto.
+  - inv H0; eauto.
+Qed.
+
+Definition index_larger {B} `{BlockType B} n (L:list B) :=
+        forall f b, get L f b -> f + n >= block_n b.
+
+Definition reset_larger {B} `{BlockType B} (L:list B) :=
+  (forall f n b b', get L f b -> get L (f - block_n b + n) b' -> n >= block_n b').
+
+Lemma sawtooth_n_tl {B} `{BlockType B} (L:list B) b n
+  : sawtooth_n n (b::L) -> sawtooth_n (S n) L \/ sawtooth_n 0 L.
+Proof.
+  unfold sawtooth_n; intros.
+  destruct L.
+  - right; split; isabsurd.
+  - destruct_prop (block_n b0 = 0).
+    + right; split.
+      * hnf; intros. eapply H0; eauto using get.
+      * intros. inv H1. eauto.
+    + left; split.
+      * hnf; intros. eapply H0; eauto using get.
+      * hnf; intros. inv H1. dcr.
+        exploit (eapply H3; eauto using get).
+        edestruct H2; eauto using get; omega.
+Qed.
+
+Lemma sawtooth_index_larger {B} `{BlockType B} n L
+: sawtooth_n n L -> index_larger n L.
+Proof.
+  general induction L. isabsurd.
+  edestruct H0.
+  hnf; intros. inv H3.
+  erewrite H2; eauto.
+  edestruct sawtooth_n_tl; eauto.
+  orewrite (S n0 + n = n0 + S n). eapply IHL; eauto.
+  exploit (eapply (IHL _ _ H4); eauto). specialize (X _ _ H8). omega.
+Qed.
+
+Definition reset_larger' {B} `{BlockType B} n' (L:list B) :=
+  (forall f n b b', get L f b -> get L (f - block_n b + n) b' -> n + n' >= block_n b').
+
+
+Lemma sawtooth_reset_larger {B} `{BlockType B} L
+: sawtooth_n 0 L -> reset_larger L.
+Proof.
+  intros; hnf; intros.
+  general induction n.
+  - simpl in *. admit.
+  - inv H1. simpl in *.
+    pose proof (sawtooth_index_larger H0 H2); eauto. omega.
+Admitted.
+
+Lemma sawtooth_drop {B} `{BlockType B} L f n b
+: sawtooth_n n L
+  -> get L f b
+  -> sawtooth_n n (drop (f - block_n b) L).
+Proof.
+  intros.
+  hnf; intros. split.
+  hnf; intros. eapply get_drop in H2. eapply get_drop in H3.
+  eapply H0; eauto. orewrite (S (f - block_n b + f0) = f - block_n b + S f0); eauto.
+  intros. hnf in H0. eapply get_drop in H2.
+Admitted.
+*)
+
+
+Lemma egalize_funs_length1 f D n F
+      : length (snd (fst (egalize_funs f D n F))) = length F.
+Proof.
+  induction F; intros; simpl; eauto.
+  erewrite <- IHF. unfold egalize_funs.
+  repeat let_pair_case_eq; subst; simpl.
+  repeat let_pair_case_eq; subst; simpl. repeat f_equal; try omega.
+Qed.
+
+Lemma egalize_funs_length2 f D n F
+      : length (snd (egalize_funs f  D n F)) + n = fst (fst (egalize_funs f  D n F)).
+Proof.
+  revert n. induction F; intros; simpl; eauto.
+  repeat let_pair_case_eq; subst; simpl.
+  rewrite app_length. rewrite <- IHF. omega.
+Qed.
+
+Lemma egalize_funs_get F f Zb sb n D s p
+: get F f (Zb, sb)
+-> get (snd (fst (egalize_funs egalize D n F))) f (p, s)
+-> let nF := egalize_funs egalize D n (drop (f+1) F) in
+    fst (egalize D (fst (fst nF)) sb) = s /\ p = Zb.
+Proof.
+  intros.
+  general induction F. inv H. simpl in *. subst nF. inv H.
+  simpl in *.
+  repeat let_case_eq. subst. simpl in *. inv H0. rewrite eq1; eauto.
+  inv H. simpl. eapply IHF; eauto.
+  repeat let_case_eq; subst; simpl in *; eauto.
+  inv H0; eauto.
+Qed.
+
+Lemma mapi_app X Y (f:nat -> X -> Y) n L L'
+: mapi_impl f n (L++L') = mapi_impl f n L ++ mapi_impl f (n+length L) L'.
+Proof.
+  general induction L; simpl; eauto.
+  - orewrite (n + 0 = n); eauto.
+  - f_equal. rewrite IHL. f_equal; f_equal. omega.
+Qed.
+
+Lemma drop_app_eq X (L L' : list X) n
+: length L = n
+  -> drop n (L ++ L') = L'.
+Proof.
+  intros; subst. orewrite (length L = length L + 0) . eapply drop_app.
+Qed.
+
+Lemma egalize_funs_get2 D F L' f Zb sb n'
+  : get F f (Zb, sb)
+    -> exists L'',
+      let h := egalize_funs egalize D n' in
+      drop (length (snd (h (drop (f + 1) F))))
+           (mapi_impl I.mkBlock n' (snd (h F))
+                      ++ L') =
+      mapi_impl I.mkBlock (length (snd (h (drop (f + 1) F))) + n')
+                (snd (egalize D
+                              (length (snd (h (drop (f + 1) F))) + n') sb)) ++
+                L''.
+Proof.
+  intros. general induction f. inv H.
+  - simpl in *.
+    repeat let_pair_case_eq; subst; simpl.
+    rewrite <- egalize_funs_length2.
+    rewrite mapi_app.
+    simpl in *.
+    rewrite <- app_assoc.
+    erewrite (drop_app_eq). eexists. rewrite Plus.plus_comm. reflexivity.
+    rewrite mapi_length; eauto.
+  - inv H; simpl in *.
+    repeat let_pair_case_eq; subst; simpl.
+    edestruct (IHf D) with (n':=n'); eauto.
+    eexists. rewrite mapi_app. rewrite <- app_assoc.
+    eapply H0.
+Qed.
+
+
+Inductive approx (L':list I.block)
+  : list nat ->  nat -> I.block -> I.block -> Prop :=
+  Approx Z s n m s' F D f L''
+  : egalize D m s = (s', F)
+    -> drop m L' = mapi_impl I.mkBlock m F ++ L''
+    -> approx L' D f (I.blockI Z s n) (I.blockI Z s' f).
+
+Inductive renestSim : I.state -> I.state -> Prop :=
+  RenestSim (E:onv val) (L:list I.block) L' L'' s n D
+  (SL:forall f b, get L f b -> exists b', get L' (nth f D 0) b' /\ approx L' (drop (f-block_n b) D) (nth f D 0) b b')
+  (ST:sawtooth L)
+  (DP:drop n L' = mapi_impl I.mkBlock n (snd (egalize D n s)) ++ L'')
+  : renestSim (L, E, s) (L', E, (fst (egalize D n s))).
+
+
+Lemma app_drop X (L L' L'':list X)
+ : L = L' ++ L''
+   -> drop (length L') L = L''.
+Proof.
+  general induction L'; simpl; eauto.
+Qed.
+
+Instance PR : ProofRelationI (params) :=
+  {
+    ParamRelI G Z Z' := Z = Z' /\ Z = G;
+    ArgRelI G VL VL' := VL = VL' /\ length VL = length G;
+    BlockRelI := fun Z b b' => length (I.block_Z b) = length Z
+                           /\ length (I.block_Z b') = length Z
+  }.
+intros. dcr; repeat subst. eauto.
+Defined.
+
+Instance bisim_progeq {S} `{StateType S} : ProgramEquivalence S S.
+constructor. eapply (paco2 (@bisim_gen S _ S _)).
+Defined.
+
+Ltac pone_step := pfold; eapply bisim'Silent; [ eapply plus2O; single_step
+                              | eapply plus2O; single_step
+                              | ].
+
+Lemma nth_drop X (L:list X) n m x
+: nth n (drop m L) x = nth (n+m) L x.
+Proof.
+  general induction m; simpl. orewrite (n + 0 = n); eauto.
+  rewrite IHm; eauto. orewrite (n + S m = S (n + m)); eauto.
+  destruct L; simpl; eauto. destruct (n + m); eauto.
+Qed.
+
+Lemma renestSim_sim r L L' E s n D L''
+      (SL:forall (f : nat) (b : I.block),
+          get L f b ->
+          exists b' : I.block,
+            get L' (nth f D 0) b' /\
+            approx L' (drop (f - block_n b) D) (nth f D 0) b b')
+      (ST:sawtooth L)
+      (DROP:drop n L' = mapi_impl I.mkBlock n (snd (egalize D n s)) ++ L'')
+  : bisim'r r (L, E, s) (L', E, fst (egalize D n s)).
+Proof.
+  revert_all. pcofix CIH.
+  intros. destruct s; simpl in *;
+            repeat let_case_eq; repeat simpl_pair_eqs; subst; simpl in *.
+  - case_eq (exp_eval E e); intros.
+    + pone_step. right. eapply CIH; eauto.
+    + pno_step.
+  - case_eq (exp_eval E e); [ intros | intros; pno_step ].
+    rewrite mapi_app in DROP. rewrite <- app_assoc in DROP.
+    case_eq (val2bool v); intros.
+    + pone_step. right. eapply CIH; eauto.
+    + pone_step. right. eapply CIH; eauto.
+      eapply app_drop in DROP. rewrite mapi_length in DROP.
+      rewrite drop_drop in DROP. rewrite plus_comm.
+      rewrite DROP. rewrite plus_comm. eauto.
+  - destruct (get_dec L (counted l)) as [[? ?]|].
+    + edestruct SL; eauto; dcr; eauto. invt approx. destruct l as [f]; simpl in *.
+      repeat let_case_eq; repeat let_pair_case_eq; simpl in * |- *; subst.
+      decide (length Z = length Y); [| pno_step; get_functional; simpl in *; eauto].
+      case_eq (omap (exp_eval E) Y); [ intros | intros; pno_step; eauto ].
+      pone_step. right. simpl. eapply CIH.
+      *  orewrite (nth f D 0 - nth f D 0 = 0); simpl; intros ? ? GET.
+         repeat rewrite drop_drop. rewrite nth_drop.
+         eapply get_drop in GET. edestruct (SL _ _ GET); dcr.
+         rewrite plus_comm. eexists; split; eauto.
+         rewrite plus_comm; eauto.
+         pose proof (sawtooth_resetting ST _ g GET).
+         simpl in *.
+         orewrite (f - n0 + (f0 - I.block_n b) = f - n0 + f0 - I.block_n b).
+         eauto.
+      * eapply (sawtooth_drop ST g).
+      * orewrite (nth f D 0 - nth f D 0 = 0). simpl.
+        eauto.
+    + pno_step; eauto.
+      admit.
+  - pno_step.
+  - case_eq (omap (exp_eval E) Y); [intros | intros; pno_step ].
+    pextern_step.
+    + eexists; split. econstructor; eauto.
+      right. eapply CIH; eauto.
+    + eexists; split. econstructor; eauto.
+      right. eapply CIH; eauto.
+  - eapply bisim'_expansion_closed;
+      [ | eapply (S_star2 EvtTau); [ econstructor | eapply star2_refl ]
+        | eapply star2_refl].
+    eapply CIH.
+    unfold I.mkBlocks in A. eapply mapi_get in A. destruct A; dcr.
+    destruct x as [Zb sb]. unfold I.mkBlock in H10; simpl in H10.
+    subst b1. simpl. orewrite (f - f = 0). simpl.
+    exploit (eapply get_length; eauto).
+    unfold extend at 1. unfold extend at 2.
+    rewrite app_nth1; eauto.
+    repeat rewrite nth_mapi; eauto. subst. simpl in *.
+    edestruct get_in_range. Focus 2.
+    eexists. split. rewrite Plus.plus_comm. eapply get_drop.
+    rewrite DP. rewrite mapi_app. repeat eapply get_app. eapply g.
+    exploit (eapply mapi_get_impl; eauto using get_getT). destruct X0 as [? [? ?]].
+    subst. eapply getT_get in g0. unfold I.mkBlock. destruct x0. simpl.
+    edestruct egalize_funs_get; try eapply H8; try eapply g0. subst p.
+
+    repeat rewrite mapi_app in DP.
+    repeat rewrite <- app_assoc in DP.
+    eapply app_drop in DP.
+    repeat rewrite mapi_length in DP.
+    rewrite drop_drop in DP.
+    rewrite egalize_funs_length1 in DP.
+    rewrite <- Plus.plus_assoc in DP. rewrite Plus.plus_comm in DP.
+
+    intros.
+    intros. edestruct (@egalize_funs_get2 (extend n F D) F) with (n':= n + length F). eassumption.
+    eapply Approx.
+    subst. eapply surjective_pairing.
+    rewrite <- egalize_funs_length2.
+    rewrite <- drop_drop. rewrite Plus.plus_comm. rewrite DP.
+    simpl in *.
+    eapply H3.
+
+    rewrite mapi_length. rewrite egalize_funs_length1; eauto.
+    unfold mapi. rewrite mapi_length; eauto.
+  - edestruct (SL _ _ H8); dcr. unfold extend.
+    repeat rewrite app_nth2; eauto.
+    unfold mapi. rewrite mapi_length. eexists x.
+    split.
+    unfold I.mkBlocks in *. unfold mapi in *. rewrite mapi_length in *. eauto.
+    unfold I.mkBlocks in *. unfold mapi in *. rewrite mapi_length in *.
+    pose proof (sawtooth_smaller ST H8). rewrite drop_length_ge. rewrite mapi_length.
+    orewrite (f - length F - I.block_n b1 = f - I.block_n b1 - length F) in H15. eauto.
+    rewrite mapi_length. simpl in *. omega.
+    unfold mapi. rewrite mapi_length. simpl in *.
+    unfold I.mkBlocks in *. unfold mapi in *. rewrite mapi_length in *. eauto.
+  - eapply sawtooth_I_mkBlocks; eauto.
+  - subst. simpl in * |- *.
+    rewrite <- egalize_funs_length2 at 1. simpl.
+    repeat rewrite mapi_app in DP. repeat rewrite <- app_assoc in DP. simpl in *.
+    eapply app_drop with (L:=drop n L') in DP. repeat rewrite mapi_length in DP. simpl in *.
+    rewrite egalize_funs_length1 in DP.
+    eapply app_drop in DP. repeat rewrite mapi_length in DP. simpl in *.
+    repeat rewrite drop_drop in DP. simpl. rewrite Plus.plus_assoc.
+    rewrite DP. simpl.
+    rewrite <- egalize_funs_length2. f_equal. f_equal. omega.
+Qed.
+
+
+
+(*
+*** Local Variables: ***
+*** coq-load-path: (("." "Lvc")) ***
+*** End: ***
+*)
